Add m_out_assign in Imp

theories/Languages/Imp.v
@@ -24,17 +24,65 @@ Inductive exp :=
 Inductive stmt :=
   | SAssign: ident -> exp -> stmt
   | SSeq : stmt -> stmt -> stmt
-  | SReturn : exp -> stmt
   | SNop : stmt.
+
+
+(** ** Equalities *)
+
+Definition type_eqb (t1 t2: type): bool :=
+  match t1, t2 with
+    | TBool, TBool => true
+  end.
+
+Definition const_eqb (c1 c2: const): bool :=
+  match c1, c2 with
+    | CBool b1, CBool b2 => Bool.eqb b1 b2
+  end.
+
+Definition binop_eqb (op1 op2: binop): bool :=
+  match op1, op2 with
+    | Bop_and, Bop_and => true
+    | Bop_or, Bop_or => true
+    | Bop_xor, Bop_xor => true
+    | _, _ => false
+  end.
+
+Fixpoint exp_eqb (e1 e2: exp): bool :=
+  match e1, e2 with
+    | EConst c1, EConst c2 => const_eqb c1 c2
+    | EInput (i1, t1), EInput (i2, t2) | EVar (i1, t1), EVar (i2, t2) =>
+      PeanoNat.Nat.eqb i1 i2 && type_eqb t1 t2
+    | EBinop op1 e11 e12, EBinop op2 e21 e22 => binop_eqb op1 op2 && exp_eqb e11 e21 && exp_eqb e12 e22
+    | _, _ => false
+  end.
+
+Fixpoint stmt_eqb (s1 s2: stmt): bool :=
+  match s1, s2 with
+    | SAssign i1 e1, SAssign i2 e2 =>  PeanoNat.Nat.eqb i1 i2 && exp_eqb e1 e2
+    | SSeq s11 s12, SSeq s21 s22 => stmt_eqb s11 s21 && stmt_eqb s12 s22
+    | SNop, SNop => true
+    | _, _ => false
+  end.
+
+
+(** ** Method *)
+
+Fixpoint is_substmt (sub s: stmt): bool :=
+  stmt_eqb sub s || match s with
+    | SAssign _ _ | SNop => false
+    | SSeq sl sr => is_substmt sub sl || is_substmt sub sr 
+  end.
 
 Record method := mk_method {
   m_name: ident;
 
   m_in: list binder;
-  m_out: type;
+  m_out: binder;
   m_vars: list binder;
 
   m_body: stmt;
+
+  m_out_assign: exists (e: exp), is_substmt (SAssign (fst m_out) e) m_body = true
 }.
 
 
@@ -73,15 +121,26 @@ Inductive sem_stmt: stack -> stmt -> stack -> Prop :=
       sem_stmt s2 st2 s3 ->
       sem_stmt s1 (SSeq st1 st2) s3
 
-  | SeReturn (s: stack) (e: exp) (v: value):
-      sem_exp s e v ->
-      sem_stmt s (SReturn e) s
-
   | SeNop (s: stack):
       sem_stmt s SNop s.
 
 
 (** ** Properties *)
+
+Fixpoint has_var (e: exp): bool :=
+  match e with
+    | EConst _ => false
+    | EInput _ => false
+    | EVar _ => true
+    | EBinop _ e1 e2 => has_var e1 || has_var e2
+  end.
+
+Fixpoint has_einput (e: exp): bool :=
+  match e with
+    | EInput _ => true
+    | EConst _ | EVar _ => false
+    | EBinop _ e1 e2 => has_einput e1 || has_einput e2
+  end.
 
 Fixpoint eval_exp (e: exp) (s: stack): option value :=
   match e with
@@ -99,14 +158,6 @@ Definition is_evaluable (e: exp) (s: stack): Prop :=
 
 
 (** ** Lemmas *)
-
-Fixpoint has_var (e: exp): bool :=
-  match e with
-    | EConst _ => false
-    | EInput _ => false
-    | EVar _ => true
-    | EBinop _ e1 e2 => orb (has_var e1) (has_var e2)
-  end.
 
 Lemma exp_no_var_is_const (e: exp):
   has_var e = false ->
@@ -132,5 +183,46 @@ Proof.
     exists (VBinop op v1 v2).
     simpl.
     rewrite H1, H2.
+    reflexivity.
+Qed.
+
+Lemma const_eqb_refl (c: const):
+  const_eqb c c = true.
+Proof.
+  destruct c.
+  - simpl.
+    rewrite Bool.eqb_reflx.
+    reflexivity.
+Qed.
+
+Lemma type_eqb_refl (typ: type):
+  type_eqb typ typ = true.
+Proof.
+  destruct typ.
+  - reflexivity.
+Qed.
+
+Lemma binop_eqb_refl (op: binop):
+  binop_eqb op op = true.
+Proof.
+  destruct op; reflexivity.
+Qed.
+
+Lemma exp_eqb_refl (e: exp):
+  exp_eqb e e = true.
+Proof.
+  induction e as [ c | (i, t) | (i, t) | op e1 IHe1 e2 IHe2].
+  - simpl.
+    apply const_eqb_refl.
+  - simpl.
+    rewrite PeanoNat.Nat.eqb_refl.
+    rewrite type_eqb_refl.
+    reflexivity.
+  - simpl.
+    rewrite PeanoNat.Nat.eqb_refl.
+    rewrite type_eqb_refl.
+    reflexivity.
+  - simpl.
+    rewrite binop_eqb_refl, IHe1, IHe2.
     reflexivity.
 Qed.
